Hide some proofs in Kuiper.SHMem, use fsti

src/lib/kuiper/Kuiper.SHMem.fst
@@ -12,20 +12,6 @@ open Kuiper.Common
 module SZ = Kuiper.SizeT
 module T = FStar.Tactics
 
-(* Description of one shared memory array "request" *)
-// TODO: Does the length really need to be nonzero?
-noeq
-inline_for_extraction
-type shmem_desc =
-  | SHArray :
-    (ty : Type0) ->
-    {| sized : Kuiper.Sized.sized ty |} ->
-    len    : SZ.t { len > 0 } ->
-    shmem_desc
-
-let is_block_array #ty #len (g:gpu_array ty len)
-  = visibility_of g == block_of
-
 //don't mark this an instance, to avoid clashing with other instances
 //for visibility_of, gpu_of
 let is_send_across_block_array
@@ -34,37 +20,8 @@ let is_send_across_block_array
   (#i #j #f #s:_)
 : is_send_across block_of (gpu_pts_to_slice a #f i j s)
 = let i : is_send_across (visibility_of a) (gpu_pts_to_slice a #f i j s)
-   = FStar.Tactics.Typeclasses.solve in
+   = Tactics.Typeclasses.solve in
   i
-
-inline_for_extraction unfold
-let c_shmem (d : shmem_desc) : Type0 =
-  match d with
-  | SHArray ty len -> gpu_array ty len
-   //would be nice to just add as is_block_array refinement here, but it messes with typeclass resolution
-
-let rec c_shmems (d : list shmem_desc) : Type0 =
-  match d with
-  | [] -> int // This could (and should) be unit, but karamel extraction gets confused with it
-  | d :: ds ->
-    c_shmem d & c_shmems ds
-
-let c_shmem_inv (#d : shmem_desc) (c:c_shmem d) : prop =
-  match d with
-  | SHArray ty len -> is_block_array #ty #len c
-
-let rec c_shmems_inv (#ds : list shmem_desc) (c:c_shmems ds) : prop =
-  match ds with
-  | [] -> True
-  | d :: ds ->
-    let c : c_shmem d & c_shmems ds = c in (* coerce *)
-    c_shmem_inv #d (fst c) /\
-    c_shmems_inv #ds (snd c)
-
-let live_c_shmem #d (c : c_shmem d) (#[T.exact (`1.0R)]f:_) : slprop =
-  match d with
-  | SHArray ty len ->
-    exists* v. gpu_pts_to_array #ty #len c #f v
 
 instance is_send_across_live_c_shmem #d (c:c_shmem d) #f (_:squash (c_shmem_inv c))
 : is_send_across block_of (live_c_shmem #d c #f)
@@ -81,33 +38,25 @@ instance is_send_across_live_c_shmem #d (c:c_shmem d) #f (_:squash (c_shmem_inv 
     in
     ff
 
-let rec live_c_shmems #ds (c : c_shmems ds) (#[T.exact (`1.0R)]f:_) : slprop =
-  match ds with
-  | [] -> emp
-  | d :: ds ->
-    let c : c_shmem d & c_shmems ds = c in (* coerce *)
-    live_c_shmem #d (fst c) #f ** live_c_shmems #ds (snd c) #f
-
 ghost
 fn unfold_live_c_shmems_nil (c : c_shmems []) (#[T.exact (`1.0R)]f:_)
-requires live_c_shmems c #f
-ensures emp
+  requires live_c_shmems c #f
+  ensures emp
 {
-  rewrite (live_c_shmems c #f)
-      as  emp
+  rewrite live_c_shmems c #f as emp;
 }
 
 ghost
 fn fold_live_c_shmems_nil (c : c_shmems []) (#[T.exact (`1.0R)]f:_)
-ensures live_c_shmems c #f
+  ensures live_c_shmems c #f
 {
-  rewrite emp as (live_c_shmems c #f);
+  rewrite emp as live_c_shmems c #f;
 }
 
 ghost
 fn unfold_live_c_shmems_cons #d #ds (c : c_shmems (d::ds)) (#[T.exact (`1.0R)]f:_)
-requires live_c_shmems c #f
-ensures live_c_shmem #d (fst c) #f ** live_c_shmems #ds (snd c) #f
+  requires live_c_shmems c #f
+  ensures live_c_shmem #d (fst c) #f ** live_c_shmems #ds (snd c) #f
 {
   rewrite (live_c_shmems c #f)
       as  (live_c_shmem #d (fst c) #f ** live_c_shmems #ds (snd c) #f)
@@ -124,8 +73,7 @@ ensures live_c_shmems c #f
 
 let rec is_send_across_live_c_shmems_ #ds (c:c_shmems ds) #f (pf:squash (c_shmems_inv c))
 : is_send_across block_of (live_c_shmems #ds c #f)
-= let open FStar.Tactics.Typeclasses in
-  match ds with
+= match ds with
   | [] -> solve #(is_send_across block_of emp)
   | d::ds ->
     let c : c_shmem d & c_shmems ds = c in (* coerce *)
@@ -139,8 +87,8 @@ instance is_send_across_live_c_shmems #ds (c:c_shmems ds) #f (pf:squash (c_shmem
 
 ghost
 fn unfold_c_shmems (#ds:_) (c:c_shmems ds) (#f:_) (desc:_)
-requires live_c_shmems c #f
-ensures FStar.Pervasives.norm [zeta; iota; delta_only [`%live_c_shmems; `%live_c_shmem; desc]] (live_c_shmems c #f)
+  requires live_c_shmems c #f
+  ensures Pervasives.norm [zeta; iota; delta_only [`%live_c_shmems; `%live_c_shmem; desc]] (live_c_shmems c #f)
 {
   reduce_with_steps (live_c_shmems c #f) [zeta; iota; delta_only [`%live_c_shmems; `%live_c_shmem; desc]];
 }
@@ -148,32 +96,28 @@ ensures FStar.Pervasives.norm [zeta; iota; delta_only [`%live_c_shmems; `%live_c
 
 ghost
 fn fold_c_shmems (#ds:_) (c:c_shmems ds) (#f:_) (desc:_)
-requires FStar.Pervasives.norm [zeta; iota; delta_only [`%live_c_shmems; `%live_c_shmem; desc]] (live_c_shmems c #f)
-ensures live_c_shmems c #f
+  requires Pervasives.norm [zeta; iota; delta_only [`%live_c_shmems; `%live_c_shmem; desc]] (live_c_shmems c #f)
+  ensures live_c_shmems c #f
 {
   norm_spec [zeta; iota; delta_only [`%live_c_shmems; `%live_c_shmem; desc]] (live_c_shmems c #f);
-  rewrite (FStar.Pervasives.norm [zeta; iota; delta_only [`%live_c_shmems; `%live_c_shmem; desc]] (live_c_shmems c #f))
+  rewrite (Pervasives.norm [zeta; iota; delta_only [`%live_c_shmems; `%live_c_shmem; desc]] (live_c_shmems c #f))
   as (live_c_shmems c #f);
 }
 
-let d_ty d : Type0 = let SHArray ty _ = d in ty
-let d_ty_sized d : Kuiper.Sized.sized (d_ty d) = let SHArray _ #s _ = d in s
-let d_len d : SZ.t = let SHArray _ len = d in len
-
 ghost
 fn unfold_live_c_shmem #d (c:c_shmem d) #f
-requires live_c_shmem c #f
-ensures exists* (s:Seq.seq (d_ty d)). gpu_pts_to_array #(d_ty d) #(d_len d) c #f s
+  requires live_c_shmem c #f
+  ensures exists* (s:Seq.seq (d_ty d)). gpu_pts_to_array #(d_ty d) #(d_len d) c #f s
 {
-   rewrite each d as (SHArray (d_ty d) #(d_ty_sized d) (d_len d));
+  rewrite each d as (SHArray (d_ty d) #(d_ty_sized d) (d_len d));
   reduce_with_steps (live_c_shmem #((SHArray (d_ty d) #(d_ty_sized d) (d_len d))) c #f)
                     [delta_only [`%live_c_shmem]; iota]
 }
 
 ghost
 fn fold_live_c_shmem #d (c:c_shmem d) #f
-requires exists* (s:Seq.seq (d_ty d)). gpu_pts_to_array #(d_ty d) #(d_len d) c #f s
-ensures live_c_shmem c #f
+  requires exists* (s:Seq.seq (d_ty d)). gpu_pts_to_array #(d_ty d) #(d_len d) c #f s
+  ensures live_c_shmem c #f
 {
   rewrite each d as (SHArray (d_ty d) #(d_ty_sized d) (d_len d));
   fold (live_c_shmem #((SHArray (d_ty d) #(d_ty_sized d) (d_len d))) c #f);
@@ -199,12 +143,12 @@ ensures
 
 ghost
 fn rec gpu_live_c_shmems_share_underspec
-    (#ds:_) (c:c_shmems ds) (#f:_) (#k:nat { k > 0 })
-requires
-  live_c_shmems c #f
-ensures
-  forall+ (_ : natlt k). live_c_shmems c #(f /. Real.of_int k)
-decreases ds
+  (#ds:_) (c:c_shmems ds) (#f:_) (#k:nat { k > 0 })
+  requires
+    live_c_shmems c #f
+  ensures
+    forall+ (_ : natlt k). live_c_shmems c #(f /. Real.of_int k)
+  decreases ds
 {
   match ds {
     [] -> {
@@ -237,11 +181,11 @@ decreases ds
 
 ghost
 fn gpu_live_c_shmem_gather_underspec
-    (#d:_) (c:c_shmem d) (#f:perm) (#k:nat { k > 0 })
-requires
-  forall+ (_ : natlt k). live_c_shmem c #(f /. Real.of_int k)
-ensures
-  live_c_shmem c #f
+  (#d:_) (c:c_shmem d) (#f:perm) (#k:nat { k > 0 })
+  requires
+    forall+ (_ : natlt k). live_c_shmem c #(f /. Real.of_int k)
+  ensures
+    live_c_shmem c #f
 {
   forevery_map #(natlt k)
     (fun _ -> live_c_shmem c #(f /. Real.of_int k))
@@ -253,12 +197,12 @@ ensures
 
 ghost
 fn rec gpu_live_c_shmems_gather_underspec
-    (#ds:_) (c:c_shmems ds) (#f:perm) (#k:nat { k > 0 })
-requires
-  forall+ (_ : natlt k). live_c_shmems c #(f /. Real.of_int k)
-ensures
-  live_c_shmems c #f
-decreases ds
+  (#ds:_) (c:c_shmems ds) (#f:perm) (#k:nat { k > 0 })
+  requires
+    forall+ (_ : natlt k). live_c_shmems c #(f /. Real.of_int k)
+  ensures
+    live_c_shmems c #f
+  decreases ds
 {
   match ds {
     [] -> {
