src/lib/kuiper/Kuiper.SHMem.fsti
@@ -1,0 +1,150 @@
+module Kuiper.SHMem
+
+#lang-pulse
+
+open Pulse.Lib.Core
+open Pulse.Lib.Pervasives
+open Kuiper.Base
+open Kuiper.Array
+open FStar.Tactics.V2
+open Kuiper.ForEvery
+open Kuiper.Common
+module SZ = Kuiper.SizeT
+module T = FStar.Tactics
+
+(* Description of one shared memory array "request" *)
+// TODO: Does the length really need to be nonzero?
+noeq
+inline_for_extraction
+type shmem_desc =
+  | SHArray :
+    (ty : Type0) ->
+    {| sized : Kuiper.Sized.sized ty |} ->
+    len    : SZ.t { len > 0 } ->
+    shmem_desc
+
+let is_block_array #ty #len (g:gpu_array ty len)
+  = visibility_of g == block_of
+
+val is_send_across_block_array
+  (#et:Type0) (#sz:_)
+  (a:gpu_array et sz { is_block_array a })
+  (#i #j #f #s:_)
+: is_send_across block_of (gpu_pts_to_slice a #f i j s)
+
+inline_for_extraction unfold
+let c_shmem (d : shmem_desc) : Type0 =
+  match d with
+  | SHArray ty len -> gpu_array ty len
+  //would be nice to just add as is_block_array refinement here, but it messes with typeclass resolution
+
+let rec c_shmems (d : list shmem_desc) : Type0 =
+  match d with
+  | [] -> int // This could (and should) be unit, but karamel extraction gets confused with it
+  | d :: ds ->
+    c_shmem d & c_shmems ds
+
+let c_shmem_inv (#d : shmem_desc) (c:c_shmem d) : prop =
+  match d with
+  | SHArray ty len -> is_block_array #ty #len c
+
+let rec c_shmems_inv (#ds : list shmem_desc) (c:c_shmems ds) : prop =
+  match ds with
+  | [] -> True
+  | d :: ds ->
+    let c : c_shmem d & c_shmems ds = c in (* coerce *)
+    c_shmem_inv #d (fst c) /\
+    c_shmems_inv #ds (snd c)
+
+let live_c_shmem #d (c : c_shmem d) (#[T.exact (`1.0R)]f:_) : slprop =
+  match d with
+  | SHArray ty len ->
+    exists* v. gpu_pts_to_array #ty #len c #f v
+
+instance val is_send_across_live_c_shmem #d (c:c_shmem d) #f (_:squash (c_shmem_inv c))
+: is_send_across block_of (live_c_shmem #d c #f)
+
+let rec live_c_shmems #ds (c : c_shmems ds) (#[T.exact (`1.0R)]f:_) : slprop =
+  match ds with
+  | [] -> emp
+  | d :: ds ->
+    let c : c_shmem d & c_shmems ds = c in (* coerce *)
+    live_c_shmem #d (fst c) #f ** live_c_shmems #ds (snd c) #f
+
+ghost
+fn unfold_live_c_shmems_nil (c : c_shmems []) (#[T.exact (`1.0R)]f:_)
+  requires live_c_shmems c #f
+  ensures emp
+
+ghost
+fn fold_live_c_shmems_nil (c : c_shmems []) (#[T.exact (`1.0R)]f:_)
+  ensures live_c_shmems c #f
+
+ghost
+fn unfold_live_c_shmems_cons #d #ds (c : c_shmems (d::ds)) (#[T.exact (`1.0R)]f:_)
+  requires live_c_shmems c #f
+  ensures live_c_shmem #d (fst c) #f ** live_c_shmems #ds (snd c) #f
+
+ghost
+fn fold_live_c_shmems_cons #d #ds (c : c_shmems (d::ds)) (#[T.exact (`1.0R)]f:_)
+  requires live_c_shmem #d (fst c) #f ** live_c_shmems #ds (snd c) #f
+  ensures live_c_shmems c #f
+
+instance val is_send_across_live_c_shmems #ds (c:c_shmems ds) #f (pf:squash (c_shmems_inv c))
+: is_send_across block_of (live_c_shmems #ds c #f)
+
+ghost
+fn unfold_c_shmems (#ds:_) (c:c_shmems ds) (#f:_) (desc:_)
+  requires live_c_shmems c #f
+  ensures FStar.Pervasives.norm [zeta; iota; delta_only [`%live_c_shmems; `%live_c_shmem; desc]] (live_c_shmems c #f)
+
+ghost
+fn fold_c_shmems (#ds:_) (c:c_shmems ds) (#f:_) (desc:_)
+  requires FStar.Pervasives.norm [zeta; iota; delta_only [`%live_c_shmems; `%live_c_shmem; desc]] (live_c_shmems c #f)
+  ensures live_c_shmems c #f
+
+let d_ty d : Type0 = let SHArray ty _ = d in ty
+let d_ty_sized d : Kuiper.Sized.sized (d_ty d) = let SHArray _ #s _ = d in s
+let d_len d : SZ.t = let SHArray _ len = d in len
+
+ghost
+fn unfold_live_c_shmem #d (c:c_shmem d) #f
+  requires live_c_shmem c #f
+  ensures exists* (s:Seq.seq (d_ty d)). gpu_pts_to_array #(d_ty d) #(d_len d) c #f s
+
+ghost
+fn fold_live_c_shmem #d (c:c_shmem d) #f
+  requires exists* (s:Seq.seq (d_ty d)). gpu_pts_to_array #(d_ty d) #(d_len d) c #f s
+  ensures live_c_shmem c #f
+
+ghost
+fn gpu_live_c_shmem_share_underspec
+    (#d:_) (c:c_shmem d) (#f:_) (#k:nat { k > 0 })
+  requires
+    live_c_shmem c #f
+  ensures
+    forall+ (_ : natlt k). live_c_shmem c #(f /. Real.of_int k)
+
+ghost
+fn gpu_live_c_shmems_share_underspec
+  (#ds:_) (c:c_shmems ds) (#f:_) (#k:nat { k > 0 })
+  requires
+    live_c_shmems c #f
+  ensures
+    forall+ (_ : natlt k). live_c_shmems c #(f /. Real.of_int k)
+
+ghost
+fn gpu_live_c_shmem_gather_underspec
+  (#d:_) (c:c_shmem d) (#f:perm) (#k:nat { k > 0 })
+  requires
+    forall+ (_ : natlt k). live_c_shmem c #(f /. Real.of_int k)
+  ensures
+    live_c_shmem c #f
+
+ghost
+fn gpu_live_c_shmems_gather_underspec
+  (#ds:_) (c:c_shmems ds) (#f:perm) (#k:nat { k > 0 })
+  requires
+    forall+ (_ : natlt k). live_c_shmems c #(f /. Real.of_int k)
+  ensures
+    live_c_shmems c #f
